\documentclass[main.tex]{subfiles}

\begin{document}
For points $A, B : \uc$, we seek to make an identification between morphisms $\ho[\uc]{A}{B}$ and functions between types $\El(A) \to \El(B)$. That is, we seek to state some directed univalence principle that allows us to identify morphisms with functions. To formalize this notion, we start by defining some canonical function:

\begin{lemma}
\label{lem:can_define_htf}
For any two $A,B : \uc$, there is a function
\begin{equation}
    \htf : \ho[\uc]{A}{B} \to (\El(A) \to \El(B)).
\end{equation}

\end{lemma}
\begin{proof}
    We begin by observing that the identity function on $\uc$,
        $$\id{\uc} : \uc \to \uc$$
    induces a covariant function $$F \defeq \lam{A : \uc}\El(A) : \uc \to \U.$$ So, by Lemma~\ref{lem:covcodiscov} the type family 
    \begin{equation}
        \label{eqn:zetaisucovid}
    C \defeq \lam{B : \uc}\El(A) \to F(B) : \uc \to \U
    \end{equation}
    is also covariant. Note that \eqref{eqn:zetaisucovid} can be restated as $C \equiv \lam{B : \uc} \El(A) \to \El(B)$. Finally, we appeal to \cref{thm:yonlemma}, the Yoneda lemma, to define $\htf$:
    \begin{align}
        \htf \defeq \\  \yon{C}{\El(A)}(\id{\El(A)})(\El(B)) \defeq\\ \lam{f}f_*(\id{\El(A)}) : \ho[\uc]{A}{B} \to (\El(A) \to \El(B)) 
    \end{align}
\end{proof}
\begin{remark}
    Note that $\htf$ behaves like a functor, so for any $f : \ho[\uc]{A}{B}$ and $g : \ho[\uc]{B}{C}$,
    \begin{align*}
        \htf(g \cdot f) : \El(A) \to \El(C) \equiv\\
        (g\cdot f)_*(\id{\El(A)}) =\\
        g_*(f_*(\id{\El(A)})) \equiv \\
        \lam{x:\El(A)}(\htf(g))((\htf(f))(x)) : \El(A) \to \El(C)
    \end{align*}
with the second equality following from \cref{lem:tptisfunctorial}. 

\end{remark}
Just as HoTT does not come equipped with tools to show idtoeqv is an equivalence, sHoTT also does not come equipped with the tools to show $\htf$
 is an equivalence. Instead, we can postulate \textit{directed univalence} as an axiom.

\begin{axiom}[Directed Univalence]
    For any points $A,B : \uc$, the function defined in Lemma~\ref{lem:can_define_htf} is an equivalence.
\end{axiom}

For points $A,B : \uc$, we can break the equivalence up into:
\begin{itemize}
    \item An introduction rule for $\ho[\uc]{A}{B}$ denoted $\dua$ for "directed univalence axiom":
    $$\dua : (\El(A) \to \El(B)) \to (\ho[\uc]{A}{B})$$
    \item An elimination rule
    $$\htf \defeq \yon{C}{\El(A)}(\id{\El(A)}) : \ho[\uc]{A}{B} \to (\El(A) \to \El(B))$$
    \item The propositional computation rule
        $$\htf(\dua(f)) = f$$
    \item The propositional uniqueness rule, which states for any $f : \ho[\uc]{A} {B}$,
    $$f = \dua(\htf(f))$$
\end{itemize}
Directed univalence also allows us to  identify identity morphisms with identity functions and composition of morphisms in $\uc$ with composition of functions, stated tersely as
\begin{align*}
    \idhom{A} = \dua(\id{\El(A)})\\
    \dua{g}\cdot\dua{f} = \dua(g \circ f).
\end{align*}
The first equality from the fact that \begin{align*}
\id{\El(A)} = \\
(\idhom{A})_*(\id{A}) \equiv \\
\htf(\idhom{A})
\end{align*} by proposition 8.16. To show the second, if we define $p \defeq \dua(f)$ and $q \defeq \dua(g)$, then
    $$\dua(g \circ f) = \dua(\htf(p) \circ \htf(q)) = \dua(\htf(p \cdot q)) = p \cdot q$$

With directed univalence, we can show that dependent transport is really just coercing a morphism of types.
\begin{lemma}
    \label{lem:tptissubst}
    For any covariant family $P : A \to \U$ and morphism $f : \ho[A]{x}{y}$,
    \begin{equation*}
        \dua(f_*) = \overline{P}(f)
    \end{equation*}
\end{lemma}
\begin{proof}
    We have the following chain of equalities:
    \begin{align*}
        \dua(f_*) \equiv \\
        \dua(\dtran{P}(f, -)) \equiv \\
        \dua(\dtran{\lam{x}\El(\overline{P}(x))}(f, -)) = \\
        \dua(\dtran{\lam{x}\El(x)}(\mapfunc{\overline{P}}f, -)) \equiv \\
        \dua(\htf(\mapfunc{\overline{P}}f)) = \\
        \mapfunc{\overline{P}}f \defeq \\
        \overline{P}(f)
    \end{align*}
    with the first following from lemma~\ref{lem:tpthomiscoethenapp} which allows us to decompose the transport of a composition into an application and a coercion. The second equality comes from the propositional uniqueness rule.
\end{proof}
We can also show that a morphism between functions is a commutative square.
\begin{lemma}
    \label{lem:covhoissq}
    For any two covariant families $F, G : A \to \U$, a morphism $h : \ho[A]{x}{y}$ and maps $f : F(x) \to G(x)$, and $g : F(y) \to G(y)$ we have the following:
    \begin{equation*}
        \ho[(\lam{x}F(x)\to G(x))h]{f}{q} \simeq g \circ h_* = h_*  \circ f
    \end{equation*}
\end{lemma}
\begin{proof}
    By directed univalence,
    \begin{equation*}
        \ho[(\lam{x}F(x)\to G(x))h]{f}{q} \simeq
        \ho[{(\lam{x}\ho[\uc]{\overline{F}(x)}{\overline{G}(x)})h}]{\dua f}{\dua g}
    \end{equation*}
    By lemma~\ref{lem:compissquare}, this is equivalent to
    \begin{equation*}
        \dua g \cdot \overline{F}(h) = \overline{G}(h) \cdot \dua f
    \end{equation*}
    which is equivalent to
    \begin{equation*}
        \dua g \cdot \dua h_* = \dua h_* \cdot \dua f
    \end{equation*}
    by lemma~\ref{lem:tptissubst}. The functorality of $\dua$ allow us to push
    this equivalence to the type
    \begin{equation*}
        \dua(g \circ h_*) = \dua(h_* \circ f).
    \end{equation*}
    From there, we can apply $\htf$ to both sides, and noting that $\htf$ and $\dua$ are inverses, extending the equivalence
    to the type $$g \circ h_* = h_* \circ f$$ by lemma ~\ref{lem:equivissurjemb}.
\end{proof}
Directed univalence also extends to characterizing dependent functions as morphisms in $\uc$.
\begin{lemma}
    \label{lem:depfuncishom}
    Given covariant type families $P : A \to \U$ and $Q : \tilde{P} \to \U$, for all $x:A$ there is an equivalence
    $$\prd{p : P(x)} Q(x,p) \simeq \sm{f : \ho[\uc]{\overline{P}(x)}{\overline{\sm{p : P(x)} Q(x,p)}}} \dua(\fst) \circ f = \idhom{\overline{P}(x)}, $$
    where $\fst : \sm{p : P(x)}Q(x,p) \to P(x)$
\end{lemma}
\begin{proof}
    We begin by noting the following equivalences
    \begin{align*}
        \sm{f : \ho[\uc]{\overline{P}(x)}{\overline{\sm{p : P(x)} Q(x,p)}}} \dua(\fst) \circ f = \idhom{\overline{P}(x)} \simeq \\
        \sm{f : P(x)\to \sm{p : P(x)} Q(x,p)}\dua(\fst) \circ \dua(f) = \idhom{\overline{P}(x)}\simeq \\
        \sm{f : P(x)\to \sm{p : P(x)} Q(x,p)}\dua(\fst \circ f) = \idhom{\overline{P}(x)}\simeq \\
        \sm{f : P(x)\to \sm{p : P(x)} Q(x,p)} \fst \circ f = \id{P(x)}
    \end{align*}
    with the first equivalence being a change of base type to an equivalence type thus following from lemma~\ref{lem:equivbaseequivtot}. The second equivalence is a result of the functorality 
    of $\dua$ and lemmas~\ref{lem:compisequiv} and~\ref{lem:equivistotequiv}. The third equivalence comes from~\ref{lem:equivissurjemb} as since $\htf$ is an equivalence, thus an embedding. Now that
    we are working with functions, we can reduce the types further:
    \begin{align*}
       \sm{f : P(x) \to \sm{p : P(x)}Q(x,p)}\fst \circ f = \id{P(x)} \simeq \\
       \sm{(f_1,f_2) : \sm{g : P(x) \to P(x)}\prd{p : P(x)}Q(x,g(p))}f_1 = \id{P(x)} \simeq\\
       \sm{f : P(x) \to P(x)}(\prd{p : P(x)}Q(x,f(p))) \times (f = \id{P(x)}) \simeq \\
       \sm{f : P(x) \to P(x)} (f = \id{P(x)})\times(\prd{p : P(x)}Q(x,f(p))) \simeq \\
       \sm{(f, p): \sm{g : P(x) \to P(x)} g = \id{P(x)}} \prd{p : P(x)}Q(x,f(p)) \simeq \\
       \prd{p : P(x)}Q(x,p)
    \end{align*}
    with the first equivalence following from the type theoretic axiom of choice, lemma~\ref{lem:ttaoc}. The second is an application of associativity, thus follows from
    lemma~\ref{lem:sigisassoc}. The third follows from the symmetry of the non-dependent pair type, lemma~\ref{lem:sigissymm}. The fourth is another application of associativity thus follows again from
    lemma~\ref{lem:sigisassoc}. Note that the base is now a contractible singleton, thus contractible by lemma~\ref{lem:contractiblesingletons}, and we can simplify the sigma type with a contractible base by lemma~\ref{lem:contractibleissimple}.
     Thus, we can get our desired equivalence by composing the two equivalences formed in this proof.
    \end{proof}
%     \begin{lemma}
%         \label{lem:commisfunarr}
%         For any covariant type families $P : A \to \U$, $Q : \prd{x : A}P(x) \to \U$, morphisms $f : \ho[A]{x}{z}$ and dependent functions
%         $\phi : \prd{p : P(x)}Q(x,p)$, $\psi : \prd{p : P(z)}Q(z,p)$, there is a map 
%         \begin{equation}
%             \label{eqn:commisfunarr}
%             f_* \circ \phi = \psi \circ f_* \to \ho[(\lam{x}\prd{p : P(x)}Q(x,p))f]{\phi}{ \psi}
%         \end{equation}
%     \end{lemma}
%     \begin{proof}
%         We start by defining a map
%         $$\zeta : \prd{p : P(x)}Q(x,p) \to (P(x) \to \sm{p : P(x)}Q(x,p))$$
%         with the defining equation
%         $$\zeta \defeq \lam{g}{p}(p, g(p)).$$
%         The codomain of \ref{eqn:commisfunarr} can be written as a morphism of sections:
%         \begin{equation*}
%             \ho[(\lam{x}(\sm{h : P(x) \to \sm{p : P(x)} Q(x,p)} \fst \circ h = \id{P(x)}))f]{(\zeta(\phi), \refl{})}{(\zeta(\psi), \refl{})}
%         \end{equation*}
%         by lemma~\ref{lem:depfuncishom}. We can then write this type as its extension type as follows:
%         \begin{equation*}
%             \exten{t : \osx}{\sm{h : P(f(t)) \to \sm{p : P(f(t))}Q(f(t), p)}\fst \circ h = \id{P(f(t))}}{\pardo}{[(\zeta(\phi), \refl{}), (\zeta(\psi), \refl{})]}
%         \end{equation*}
%         Noting that this type is a "product of sigmas", we can use the type theoretical axiom of choice, lemma ~\ref{lem:taocwet}, to write it as a "sigma of products":
%         \begin{equation}
%             \label{eqn:commisfunarr1}
%             \sm{(h : \ho[(\lam{x} P(x) \to \sm{p : P(x)}Q(x,p)))f]{\zeta(\phi)}{\zeta(\psi)}}\exten{t : \osx}{\fst \circ h(t) = \id{P(f(t))}}{\pardo}{[\refl{}, \refl{}]}.
%         \end{equation}
%         We aim to inhabit~(\ref{eqn:commisfunarr1}). Let $h : f_* \circ \phi = \psi \circ f_*$. For any $p : P(x)$, we can construct a term
%         $$h \defeq (\refl{}, \happly(h)(p)) : (f_*(p), (f_* \circ \phi)(p) ) = (f_*(p), \psi( f_*(p)))$$
%         Note that $(f_*(p), \psi( f_*(p))) \equiv (\lam{p}(p, \psi(p)))(f_*(p))$. In conjunction with lemma~\ref{cor:tptinsigma}, there is a term
%         $$h' : f_* \circ (\lam{p}(p, \phi(p)))  = (\lam{p}(p, \psi(p)))\circ f_*, $$ 
%         which by lemma~\ref{lem:compissquare} induces a term
%         $$\bar{h} : \ho[(\lam{x} P(x) \to \sm{p : P(x)}Q(x,p))f]{\zeta(\phi)}{\zeta(\psi)},$$ noting the covariance of
%         $\lam{x}\sm{p:P(x)}Q(x,p)$ by lemma~\ref{lem:covdomcovcodiscov}, that is represented by the diagram
%     % https://q.uiver.app/#q=WzAsNCxbMCwwLCJQKHgpIl0sWzAsMiwiUCh5KSJdLFszLDAsIlxcc217cDpQKHgpfVEoeCxwKSJdLFszLDIsIlxcc217cDpQKHkpfVEoeSxwKSJdLFswLDIsIlxcemV0YShcXHBoaSkiXSxbMSwzLCJcXHpldGEoXFxwc2kpIl0sWzAsMSwiUChmKSIsMV0sWzIsMywiXFxzbXtwOlAoZil9UShmLHApIiwxXV0=
%     \[\begin{tikzcd}
%         {P(x)} &&& {\sm{p:P(x)}Q(x,p)} \\
%         \\
%         {P(y)} &&& {\sm{p:P(y)}Q(y,p)}
%         \arrow["{\zeta(\phi)}", from=1-1, to=1-4]
%         \arrow["{P(f)}"{description}, from=1-1, to=3-1]
%         \arrow["{\sm{p:P(f)}Q(f,p)}"{description}, from=1-4, to=3-4]
%         \arrow["{\zeta(\psi)}", from=3-1, to=3-4]
%     \end{tikzcd}\]
%         Note here that the horizontal represents a type theoretic function, while the verticals represent simplicial morphisms.
%         We can pointwise compose $\bar{h}$ with the term $\lam{t}{p}\fst(p):\ho[(\lam{x} (\sm{p : P(x)}Q(x,p)) \to P(x))f]{\fst}{\fst}$
%         which is represented by the diagram
%     % https://q.uiver.app/#q=WzAsNCxbMCwwLCJcXHNte3A6UCh4KX1RKHgscCkiXSxbMCwyLCJcXHNte3A6UCh5KX1RKHkscCkiXSxbMiwwLCJQKHgpIl0sWzIsMiwiUCh5KSJdLFswLDEsIlxcc217cDpQKGYpfVEoZixwKSIsMV0sWzAsMiwiXFxmc3QiLDFdLFsxLDMsIlxcZnN0IiwxXSxbMiwzLCJQKGYpIiwxXV0=
%     \[\begin{tikzcd}
%         {\sm{p:P(x)}Q(x,p)} && {P(x)} \\
%         \\
%         {\sm{p:P(y)}Q(y,p)} && {P(y)}
%         \arrow["\fst"{description}, from=1-1, to=1-3]
%         \arrow["{\sm{p:P(f)}Q(f,p)}"{description}, from=1-1, to=3-1]
%         \arrow["{P(f)}"{description}, from=1-3, to=3-3]
%         \arrow["\fst"{description}, from=3-1, to=3-3]
%     \end{tikzcd}\]    
%     to yield a term 
%         $$\kappa \defeq \lam{t}\fst \circ \bar{h}(t) : \ho[(\lam{x} P(x) \to P(x))f]{\id{P(x)}}{\id{P(y)}},$$ represented by the diagram
%     % https://q.uiver.app/#q=WzAsNCxbMCwwLCJQKHgpIl0sWzAsMiwiUCh5KSJdLFsyLDAsIlAoeCkiXSxbMiwyLCJQKHkpIl0sWzAsMSwiUChmKSIsMV0sWzAsMiwiXFxpZHtQKHgpfSIsMV0sWzIsMywiUChmKSIsMV0sWzEsMywiXFxpZHtQKHkpfSIsMV1d
%     \[\begin{tikzcd}
%         {P(x)} && {P(x)} \\
%         \\
%         {P(y)} && {P(y)}
%         \arrow["{\id{P(x)}}"{description}, from=1-1, to=1-3]
%         \arrow["{P(f)}"{description}, from=1-1, to=3-1]
%         \arrow["{P(f)}"{description}, from=1-3, to=3-3]
%         \arrow["{\id{P(y)}}"{description}, from=3-1, to=3-3]
%     \end{tikzcd}\]
%         Directed univalence allows us to turn this morphism-function amalgamation digram into a pure morphism diagram. That is, there is a term
%         \begin{equation}
%             \label{eqn:duacommisarr}
%             \lam{t}\dua(\kappa(t)) : \ho[{(\lam{x} \ho[\uc]{P(x)}{P(x)})f}]{\idhom{P(x)}}{\idhom{P(y)}}
%         \end{equation}
%         represented by the diagram
%         \[\begin{tikzcd}
%         {P(x)} && {P(x)} \\
%         \\
%         {P(y)} && {P(y)}
%         \arrow["{\idhom{P(x)}}"{description}, from=1-1, to=1-3]
%         \arrow["{P(f)}"{description}, from=1-1, to=3-1]
%         \arrow["{P(f)}"{description}, from=1-3, to=3-3]
%         \arrow["{\idhom{P(y)}}"{description}, from=3-1, to=3-3]
%     \end{tikzcd}\]
%         We also make note of the fact that there is an "identity term" that inhabits the same type as \ref{eqn:duacommisarr}:
%         $$\lam{t}\idhom{P(f(t))} : \ho[{(\lam{x} \ho[\uc]{P(x)}{P(x)})f}]{\idhom{P(x)}}{\idhom{P(y)}}.$$
%         Thus, by lemma \todo{show that squares with the same side are equal in a segal type}, there is an inhabitant of the type
%         $$\lam{t}\dua(\kappa(t)) = \lam{t}\idhom{P(f(t))}.$$
%         This is equivalently typed as 
%         $$\kappa = \lam{t}\id{P(f(t))} : \exten{t:\osx}{ \fst \circ \bar{h}(t) = \id{P(f(t))}}{\pardo}{[\refl{}, \refl{}]}$$
%         Or, by unraveling definitional equalities:
%         $$\lam{t}\fst \circ \bar{h}(t) = \lam{t}\id{P(f(t))}.$$
%         This induces an inhabitant of the type 
%         $$ \exten{t:\osx}{ \fst \circ \bar{h}(t) = \id{P(f(t))}}{\pardo}{[\refl{}, \refl{}]}$$
%         as desired.
%     \end{proof}
    
\end{document}